Fix verification of shallow embedding against spec
I just brought it back to the point it was before, so there's still one
`cheat`.

With regard to whether this has run into the same performance issues as
SPI with `i2c_combs_flat`: it's worse than before, but not _too_ bad. It
used to be 745 lines and is now 2674 lines, whereas
`spi_host_combs_flat` is 19732 lines.

That's still been enough to cause _some_ performance issues, though -
there are a couple steps which take a few minutes. I could probably have
improved that, but it's still just about short enough to tolerate for
now.

I also:
- Fixed some out-of-order processes in the shallow embedding, and added
  a check that they're sorted (using a piece of Lutsig).
- Moved some stuff from RegsComm to Mappings so that changing Core
  doesn't cause a rebuild of Circuit.

util/gen_mappings.py
@@ -8,7 +8,16 @@ from reggen.field import Field
 from reggen.register import Register
 from reggen.window import Window
 
-from .common import entries, ip, name, new_field_value, reg_value, regs
+from .common import (
+    addr_width,
+    entries,
+    ip,
+    name,
+    new_field_value,
+    reg_value,
+    regs,
+    windows,
+)
 
 
 def oracle_field_value(entry: Register, field: Field):
@@ -110,12 +119,43 @@ def reg_st_upd_assn(reg: Register):
       |>;"""
 
 
+def hwext_read_rel_exp():
+    if any(
+        reg.hwext and field.swaccess.allows_read()
+        for reg in regs
+        for field in reg.fields
+    ):
+        return " /\\\n  ".join(
+            f"hw2reg.{name(reg)}.{name(field)}_d = {ip.name}_get_{name(reg)}_{name(field)} st"
+            for reg in regs
+            for field in reg.fields
+            # TODO: why is this an `any`? shouldn't it just be field.swaccess.allows_read?
+            if reg.hwext and any(field.swaccess.allows_read() for field in reg.fields)
+        )
+    else:
+        return "T"
+
+
+def win_read_rel_exp():
+    if len(windows) == 0:
+        return "T"
+    else:
+        return " /\\\n  ".join(
+            rf"""(!nb offset.
+    cheshire_req_rel (SOME (nb, offset, NONE)) (buses.req.{name(window)} with addr := (({addr_width - 1} >< 0) buses.req.{name(window)}.addr: {addr_width} word))
+    /\ buses.rsp.{name(window)}.ready
+    ==> buses.rsp.{name(window)}.error
+    \/ buses.rsp.{name(window)}.rdata = {ip.name}_{name(window)}_read st nb offset)"""
+            for window in windows
+        )
+
+
 mappings = f"""\
 open HolKernel Parse boolLib bossLib;
-open BasicProvers;
-open alignmentTheory;
+open BasicProvers wordsLib;
+open alignmentTheory wordsTheory;
 open ffiTheory;
-open {ip.name}CoreTheory {ip.name}RegsTheory;
+open cheshireCircuitTheory cheshireMiscTheory cheshireOracleTheory {ip.name}CoreTheory {ip.name}RegsTheory {ip.name}RegsCommTheory;
 
 val _ = new_theory("{ip.name}Mappings");
 
@@ -153,6 +193,145 @@ Definition {ip.name}_addrs_def:
   (* TODO: I think sh_memaddrs is supposed to only contain word-aligned addresses (which is, rather counterintuitively, what byte_align does), but we should double-check. *)
   {ip.name}_addrs = {{{"; ".join(f"byte_align {hex(reg.offset)}w" for reg in regs)}}}
 End
+
+Definition {ip.name}_hwext_read_rel_def:
+  {ip.name}_hwext_read_rel (st: {ip.name}_state) (hw2reg: {ip.name}_hw2reg) <=>
+  (* TODO: we probably shouldn't be including write-only fields in a hwext struct
+   * which happens to have other readable fields here? *)
+  {hwext_read_rel_exp()}
+End
+
+Theorem {ip.name}_hwext_read_rel_fnums:
+  {ip.name}_hwext_read_rel (st with fnums := fnums) = {ip.name}_hwext_read_rel st
+Proof
+  irule EQ_EXT >> simp [{ip.name}_hwext_read_rel_def{"".join(f", {ip.name}_get_{name(reg)}_{name(field)}_def" for reg in regs for field in reg.fields if reg.hwext and field.swaccess.allows_read())}]
+QED
+
+Definition {ip.name}_win_read_rel_def:
+  {ip.name}_win_read_rel (st: {ip.name}_state) (buses: {ip.name}_win_buses) <=>
+  {win_read_rel_exp()}
+End
+
+Theorem {ip.name}_win_read_rel_fnums:
+  {ip.name}_win_read_rel (st with fnums := fnums) = {ip.name}_win_read_rel st
+Proof
+  irule EQ_EXT >> simp [{ip.name}_win_read_rel_def{"".join(f", {ip.name}_{name(window)}_read_def" for window in windows)}]
+QED
+
+(* This probably shouldn't go here but I don't want to create a whole new file
+ * just for this. *)
+Theorem {ip.name}_tick_hwro_unchanged:
+  {ip.name}_tick notif st = INR st' ==>
+  {" /\\\n  ".join(f"st'.regs.{name(reg)}.{name(field)} = st.regs.{name(reg)}.{name(field)}" for reg in regs for field in reg.fields if not reg.hwext and not field.hwaccess.allows_write())}
+Proof
+  pure_rewrite_tac [{ip.name}_tick_def]
+  >> disch_then (assume_tac o GSYM)
+  >> fs []
+  >> rpt (pairarg_tac >> fs [])
+  >> rpt IF_CASES_TAC
+  >> simp []
+QED
+
+Theorem nb_wstrb:
+  (!i. word_bit i (wstrb: word4) <=> i < nb) /\\ n + 1 = dimindex (:'b) ==>
+  (((n >< 0) wstrb: 'b word) = -1w <=> nb > n)
+Proof
+  rpt strip_tac
+  >> full_simp_tac (boss_ss () ++ fcpLib.FCP_ss) [arithmeticTheory.GREATER_DEF, word_bit_def, word_extract_def, WORD_NEG_1_T, w2w, word_bits_def, Cong AND_CONG, arithmeticTheory.LE_LT1]
+  >> iff_tac
+  >> simp []
+QED
+
+val nb_wstrb_insts = [1, 2, 3, 4] |> map (fn bits =>
+  let
+    val all_ones_val = EVAL (wordsSyntax.mk_wordii (1, bits) |> wordsSyntax.mk_word_2comp);
+  in
+    nb_wstrb
+      |> INST [``n: num`` |-> numSyntax.term_of_int (bits - 1)]
+      |> INST_TYPE [``:'b`` |-> fcpSyntax.mk_int_numeric_type bits]
+      |> SRULE [all_ones_val]
+  end);
+
+Triviality GT_GE1:
+  (a: num) > b <=> a >= b + 1
+Proof
+  decide_tac
+QED
+
+Theorem {ip.name}_req_error_{ip.name}_write:
+  cheshire_req_rel (SOME (nb, offset, SOME wdata)) req ==>
+  (ISL ({ip.name}_write st nb offset wdata) <=> {ip.name}_req_error req /\\ ~{ip.name}_win_addr offset)
+Proof
+  simp [cheshire_req_rel_write]
+  >> rpt strip_tac
+  >> asm_simp_tac std_ss [{ip.name}_write_def, dimword_def, dimindex_{addr_width}, GSYM eq_n2w_iff_w2n_eq]
+  >> rpt TOP_CASE_TAC
+  >> simp [{ip.name}_win_addr_def, {ip.name}_req_error_def]
+  >> dep_rewrite.DEP_REWRITE_TAC nb_wstrb_insts
+  >> fs [GT_GE1]
+QED
+
+Theorem {ip.name}_req_error_{ip.name}_read:
+  cheshire_req_rel (SOME (nb, offset, NONE)) req ==>
+  (ISL ({ip.name}_read st nb offset) <=> {ip.name}_req_error req /\\ ~{ip.name}_win_addr offset)
+Proof
+  simp [cheshire_req_rel_read]
+  >> rpt strip_tac
+  >> simp [{ip.name}_read_def, GSYM eq_n2w_iff_w2n_eq]
+  >> rpt IF_CASES_TAC
+  >> simp [{ip.name}_win_addr_def, {ip.name}_req_error_def]
+QED
+
+Theorem cheshire_req_{ip.name}_req_error:
+  cheshire_req_rel req_m req_c ==>
+  (ISL (cheshire_req {ip.name}_read {ip.name}_write st req_m) <=> {ip.name}_req_error req_c /\\ ~{ip.name}_win_addr (w2n req_c.addr))
+Proof
+  rpt strip_tac
+  >> simp [cheshire_req_def]
+  >> rpt TOP_CASE_TAC
+  >- fs [cheshire_req_rel_def, {ip.name}_req_error_def]
+  >- fs [ISL_SUM_MAP, cheshire_req_rel_def, {ip.name}_req_error_{ip.name}_read]
+  >- fs [ISL_SUM_MAP, cheshire_req_rel_def, {ip.name}_req_error_{ip.name}_write]
+QED
+
+Theorem {ip.name}_write_{ip.name}_hwext_notif_rel:
+  cheshire_req_rel (SOME (nb, offset, SOME wdata)) req /\\
+  {ip.name}_write st nb offset wdata = INR (_, notif) ==>
+  {ip.name}_hwext_notif_rel notif req
+Proof
+  simp [cheshire_req_rel_write]
+  >> pure_rewrite_tac [{ip.name}_write_def]
+  >> rpt TOP_CASE_TAC
+  >> rpt strip_tac
+  >> fs [{ip.name}_hwext_notif_rel_def, {ip.name}_req_error_def, eq_n2w_iff_w2n_eq, Excl "w2n_eq_0"]
+  >> simp [GSYM eq_n2w_iff_w2n_eq]
+  >> dep_rewrite.DEP_REWRITE_TAC nb_wstrb_insts
+  >> gvs []
+QED
+
+Theorem {ip.name}_read_{ip.name}_hwext_notif_rel:
+  cheshire_req_rel (SOME (nb, offset, NONE)) req /\\
+  {ip.name}_read st nb offset = INR (notif, _) ==>
+  {ip.name}_hwext_notif_rel notif req
+Proof
+  simp [cheshire_req_rel_read]
+  >> pure_rewrite_tac [{ip.name}_read_def]
+  >> rpt TOP_CASE_TAC
+  >> rpt strip_tac
+  >> gvs [{ip.name}_hwext_notif_rel_def, {ip.name}_req_error_def, eq_n2w_iff_w2n_eq, Excl "w2n_eq_0"]
+QED
+
+Theorem cheshire_req_{ip.name}_hwext_notif_rel:
+  cheshire_req_rel req_m req_c /\\
+  cheshire_req {ip.name}_read {ip.name}_write st req_m = INR (_, notif, _) ==>
+  {ip.name}_hwext_notif_rel notif req_c
+Proof
+  rpt strip_tac
+  >> drule_then strip_assume_tac cheshire_req_INR_cases
+  >- fs [cheshire_req_rel_def, {ip.name}_hwext_notif_rel_def, {ip.name}_req_error_def]
+  >- (fs [] >> drule_all {ip.name}_read_{ip.name}_hwext_notif_rel >> simp [])
+  >- (fs [] >> drule_all {ip.name}_write_{ip.name}_hwext_notif_rel >> simp [])
+QED
 
 val _ = export_theory();
 """
