i2c/i2cCircuitStateScript.sml
@@ -1,5 +1,5 @@
 open HolKernel Parse boolLib bossLib;
-open i2cCoreTheory i2cRegsTheory i2cRegsCommTheory;
+open i2cRegsTheory i2cRegsCommTheory;
 
 val _ = new_theory "i2cCircuitState";
 
@@ -262,93 +262,5 @@ Overload stretchAddr = “39w : 6 word”;
 Overload stretchTx = “40w : 6 word”;
 Overload stretchTxSetup = “41w : 6 word”;
 Overload stretchAcqFull = “42w : 6 word”;
-
-Definition encode_fsm_def:
-  encode_fsm (machine: fsmState) =
-  case machine of
-    Idle => idle
-  | Active => active
-  | Transmitting ClockLow => clockLow
-  | Transmitting ClockPulse => clockPulse
-  | Transmitting HoldBit => holdBit
-  | Transmitting ClockLowAck => clockLowAck
-  | Transmitting ClockPulseAck => clockPulseAck
-  | Transmitting HoldDevAck => holdDevAck
-  | Receiving ReadClockLow => readClockLow
-  | Receiving ReadClockPulse => readClockPulse
-  | Receiving ReadHoldBit => readHoldBit
-  | Receiving HostClockLowAck => hostClockLowAck
-  | Receiving HostClockPulseAck => hostClockPulseAck
-  | Receiving HostHoldBitAck => hostHoldBitAck
-  | Starting SetupStart => setupStart
-  | Starting HoldStart => holdStart
-  | Starting ClockStart => clockStart
-  | Stopping ClockStop => clockStop
-  | Stopping SetupStop => setupStop
-  | Stopping HoldStop => holdStop
-  | PopFmtFifo => popFmtFifo
-End
-
-Definition fifo_rel_def:
-  (fifo_rel [] (circuit : 'a word -> 'b) (rptr : 'c word) wptr ⇔ rptr = wptr)
-∧ (fifo_rel (w :: ws) circuit rptr wptr ⇔
-     ((word_bit (dimindex(:'c) - 1) rptr = word_bit (dimindex(:'c) - 1) wptr) ⇒ wptr >+ rptr)
-   ∧ ((word_bit (dimindex(:'c) - 1) rptr ≠ word_bit (dimindex(:'c) - 1) wptr) ⇒
-      ((dimindex(:'a) - 1 >< 0) wptr : 'a word) <=+ ((dimindex(:'a) - 1 >< 0) rptr :'a word))
-   ∧ (circuit $ ((dimindex(:'a) - 1 >< 0) rptr : 'a word) = w)
-   ∧ fifo_rel ws circuit (rptr + 1w) wptr)
-End
-
-Definition core_sim_rel_def:
-  core_sim_rel (machine : i2c_state) (circuit: i2c_circuit_state) =
-  ( fifo_rel machine.rx_fifo circuit.rx_fifo_regfile circuit.rx_fifo.rptr circuit.rx_fifo.wptr
-  ∧ fifo_rel machine.fmt_fifo circuit.fmt_fifo_regfile circuit.fmt_fifo.rptr circuit.fmt_fifo.wptr
-  ∧ encode_fsm (machine.fsm_state) = circuit.fsm_state
-  ∧ machine.counter = circuit.counter
-  ∧ machine.pend_restart = circuit.pend_restart
-  ∧ machine.trans_started = circuit.trans_started
-  ∧ machine.bit_index = circuit.bit_index
-  ∧ machine.stretch_idle_cnt = circuit.stretch_idle_cnt
-  ∧ machine.byte_index = circuit.byte_index
-  ∧ machine.read_byte = circuit.read_byte
-  ∧ machine.scl_rx_val = circuit.scl_rx_val
-  ∧ machine.sda_rx_val = circuit.sda_rx_val
-  ∧ machine.regs = circuit.regs
-  )
-End
-
-Definition i2c_core_state_rel_def:
-
-  (* mstate = model state, cstate = circuit state *)
-  i2c_core_state_rel (mstate: i2c_state) (cstate: i2c_circuit_state) <=>
-    i2c_hwext_read_rel mstate cstate.hw2reg /\
-    i2c_win_read_rel mstate cstate.win_buses /\
-    (* We shouldn't really be assuming this: it's true for I2C and SPI, but in
-     * general it should be perfectly fine for an access to take more than 1 cycle
-     * to complete.
-     *
-     * Right now, though, the structure of our model assumes that an access will
-     * never take more than one cycle, and I don't want to deal with fixing that
-     * just yet; besides, much of the work of fixing this would go towards Cheshire-
-     * specific code, when I don't think it's likely that we're going to find a
-     * Cheshire peripheral which doesn't respond immediately. *)
-    i2c_win_ready cstate.win_buses /\
-    core_sim_rel mstate cstate
-End
-
-Definition i2c_state_rel_def:
-  i2c_state_rel (mstate: i2c_state) (cstate: i2c_circuit_state) <=>
-    mstate.regs = cstate.regs /\
-    i2c_notif_rel mstate.buffered_notif cstate.reg2hw /\
-    i2c_core_state_rel mstate cstate
-End
-
-Theorem i2c_state_rel_fnums:
-  i2c_state_rel (st with fnums := fnums) = i2c_state_rel st
-Proof
-  irule EQ_EXT
-  >> simp [i2c_state_rel_def, i2c_notif_rel_def, i2c_core_state_rel_def, i2c_hwext_read_rel_def, i2c_win_read_rel_def, core_sim_rel_def]
-  >> simp [i2c_get_status_fmtfull_def, i2c_get_status_rxfull_def, i2c_get_status_fmtempty_def, i2c_get_status_hostidle_def, i2c_get_status_targetidle_def, i2c_get_status_rxempty_def, i2c_get_status_txfull_def, i2c_get_status_acqfull_def, i2c_get_status_txempty_def, i2c_get_status_acqempty_def, i2c_get_rdata_rdata_def, i2c_get_fifo_status_fmtlvl_def, i2c_get_fifo_status_txlvl_def, i2c_get_fifo_status_rxlvl_def, i2c_get_fifo_status_acqlvl_def, i2c_get_val_scl_rx_def, i2c_get_val_sda_rx_def, i2c_get_acqdata_abyte_def, i2c_get_acqdata_signal_def]
-QED
 
 val _ = export_theory ();
